\documentclass[10pt]{article}
\usepackage[utf8]{inputenc}
\usepackage[italian]{babel}
\usepackage{multicol}
\usepackage[bookmarks]{hyperref}
\usepackage[a4paper, total={18cm, 25cm}]{geometry}
\usepackage{amsfonts}
\begin{document}
\title{Eserciziario di Analisi Matematica}
\author{Federico Matteoni}
\date{ }
\renewcommand*\contentsname{Indice}

\maketitle
\tableofcontents
\pagebreak
\section{Derivate}
	\begin{multicols}{2}
		\begin{enumerate}
			\item 
		\end{enumerate}
	\end{multicols}
\pagebreak
\section{Integrali}
	\begin{multicols}{2}
		\begin{enumerate}
			\item $$\int \frac{1}{x\cdot\ln(x)\cdot(\ln(\ln(x))))^2}\, dx = -\frac{1}{\ln(\ln(x))} + c$$
			\item $$\int \frac{x + 2}{\sqrt{1 - x^2}}\, dx = 2\arcsin(x) - \sqrt{1 - x^2} + c $$
		\end{enumerate}
	\end{multicols}
\pagebreak
\section{Limiti}
	\begin{multicols}{2}
		\begin{enumerate}
			\item $$\lim_{x\to+\infty} \frac{x^4 - x^3 + 1}{\sqrt{x} + x^2 - x^3} = -\infty$$
			\item $$\lim_{x\to0} \frac{x^3 - x^2 + 4x}{x^5 - x} = -4$$
			\item $$\lim_{x\to1^+} \frac{x^4 - x^3 + 1}{1 - x^3} = \infty$$
			\item $$\lim_{x\to0} \frac{x\cdot\sin^2(8x)}{(1 - \cos(x))\ln(1 + \tan(x))} = 128$$
			\item $$\lim_{x\to1} \frac{x^3 - 3x + 2}{x^2 - 6x + 5} = 0$$
			\item $$\lim_{x\to2} \frac{3 - \sqrt{5x - 1}}{4 - x^2} = \frac{5}{24}$$
			\item $$\lim_{x\to+\infty} \frac{x^2 - 3x^4}{2x^2 - x + 4x^4} = -\frac{3}{4}$$
			\item $$\lim_{x\to+\infty} \frac{x^2 - 2}{x^2 - 2x + 1} = 0$$
			\item $$\lim_{x\to+\infty} \frac{x + \sqrt{x^2 + 8}}{2x + 1} = 1$$
			\item $$\lim_{x\to-\infty} \frac{\sqrt[3]{3x^3 - 2x^2 + 5}}{2x + \sqrt{x^2 - 1}} = \sqrt[3]{3}$$
			\item $$\lim_{x\to+\infty} \frac{2 + \cos(x)}{2x + \sin(x)} = 0$$
			\item $$\lim_{x\to+\infty} \frac{2^x + (\frac{27}{10})^x}{x + e^x} = 0$$
			\item $$\lim_{x\to+\infty} e^x - x^x = -\infty (x = e^{\ln(x)})$$
		\end{enumerate}
	\end{multicols}
\pagebreak
\section{Equazioni differenziali}
	\begin{multicols}{2}
		\begin{enumerate}
			\item 
		\end{enumerate}
	\end{multicols}
\end{document}